TestingMachine.v
@@ -1,18 +1,9 @@
 Set Warnings "-notation-overridden,-parsing,-deprecated-hint-without-locality".
-From Stdlib Require Import Strings.String.
-From Stdlib Require Import Bool.Bool.
-From Stdlib Require Import Arith.Arith.
-From Stdlib Require Import Arith.EqNat.
-From Stdlib Require Import Arith.PeanoNat. Import Nat.
-From Stdlib Require Import Lia.
-From Stdlib Require Import List. Import ListNotations.
-From Stdlib Require Import Classes.EquivDec.
-From Stdlib Require Import String.
-
-Set Default Goal Selector "!".
 
 From QuickChick Require Import QuickChick Tactics.
 Import QcNotation QcDefaultNotation. Open Scope qc_scope.
+
+From Stdlib Require Import List. Import ListNotations.
 
 Require Export ExtLib.Structures.Monads.
 Require Import ExtLib.Structures.Traversable.
@@ -20,31 +11,31 @@ Require Import ExtLib.Data.List.
 Require Import ExtLib.Data.Monads.OptionMonad.
 Import MonadNotation. Open Scope monad_scope.
 
-From SECF Require Import TestingLib.
-From SECF Require Import Utils.
-From SECF Require Import ListMaps MapsFunctor.
-From SECF Require Import MiniCET Machine.
-From SECF Require Import TestingMiniCET.
-From SECF Require Import sflib.
+From SECF Require Import 
+  Utils
+  ListMaps
+  MapsFunctor
+  MiniCET
+  Machine
+  TaintTracking
+  TestingLib.
 
 Import MonadNotation.
 Local Open Scope monad_scope.
-
-(*! Section testing_machine_ETE *)
-
-Inductive ty : Type := | TNum.
-
-Derive (Arbitrary, Shrink) for ty.
-Derive Show for ty.
-
-Definition ty_eqb (x y: ty) := match x, y with
-                               | TNum, TNum => true
-                               end.
-
 (* Executable Semantics for testing *)
 
-Module MCC := MachineCommon(ListTotalMap).
-Import MCC.
+Module Import MCC := MachineCommon(ListTotalMap).
+Module Import TS := TestingStrategies(MCC).
+Module Import TT := TaintTracking(MCC).
+Module Import SC := SimCommon(ListTotalMap).
+
+Definition gen_dbr : G dir :=
+  b <- arbitrary;; ret (DBranch b).
+
+Definition gen_dcall (pst: list nat) : G direction :=
+  l <- (elems_ 0 (proc_hd pst));; ret (DCall (l, 0)).
+
+Derive Show for direction.
 
 (* Find the condition that make machine_prog total function. I guess its wf. *)
 (* Port existing tests from TestingMiniCET and Define some sanity checks for machine langauge. *)
@@ -76,3 +67,198 @@ Definition test_machine_branch_from_wf_minicet :=
   wf_jmp (machine_prog harden))).
 
 (*! QuickChick test_machine_branch_from_wf_minicet. *)
+
+Print cfg.
+
+Class Transform (A : Type) := mkTransform {
+  transform : A -> A
+}.
+
+Instance MachineProg : Transform prog := {
+  transform p := machine_prog p
+}.
+
+Instance MachineMem : Transform mem := {
+  transform m := machine_mem m
+}.
+
+Instance MachineReg : Transform reg := {
+  transform r := machine_rctx r
+}.
+
+Instance TransformPair {A B : Type} `{Transform A} `{Transform B}: Transform (A * B) := {
+  transform x := let '(a, b) := x in (transform a, transform b)
+}.
+
+Instance TransformTuple {A B C : Type} `{Transform A} `{Transform B} `{Transform C}: Transform (A * B * C) := {
+  transform '(a, b, c) := (transform a, transform b, transform c)
+}.
+
+Definition stuck_free (f : nat) (p : prog) (c: cfg) : exec_result :=
+  let '(pc, rs, m, ts) := c in
+  let tpc := [] in
+  let trs := ([], map (fun x => (x,[@inl reg_id mem_addr x])) (map_dom (snd rs))) in
+  let tm := init_taint_mem m in
+  let ts := [] in
+  let tc := (tpc, trs, tm, ts) in
+  let ist := (c, tc, []) in
+  steps_taint_track f p ist [].
+
+Definition load_store_trans_stuck_free `{Transform (prog * mem * reg)} := (
+  forAll (gen_prog_wt_with_basic_blk 3 8) (fun '(c, tm, pst, p) =>
+  forAll (gen_reg_wt c pst) (fun rs =>
+  forAll (gen_wt_mem tm pst) (fun m =>
+  let p := transform_load_store_prog c tm p in
+  let '(p, m, rs)  := transform (p, m, rs) in 
+  let icfg := (ipc, rs, m, istk) in
+  let r1 := stuck_free 1000 (machine_prog p) icfg in
+  match r1 with
+  | ETerm st os => checker true
+  | EOutOfFuel st os => checker tt
+  | EError st os => printTestCase (show p ++ nl) (checker false)
+  end)))).
+
+QuickChick load_store_trans_stuck_free.
+(* +++ Passed 10000 tests (6286 discards) *)
+
+Definition unused_var_no_leak `{Transform (prog * mem * reg)} := (
+  forAll gen_prog_and_unused_var (fun '(c, tm, pst, p, unused_var) =>
+  forAll (gen_reg_wt c pst) (fun rs =>
+  forAll (gen_wt_mem tm pst) (fun m =>
+  let p := transform_load_store_prog c tm p in
+  let '(p, m, rs) := transform (p, m, rs) in
+  let icfg := (ipc, rs, m, istk) in
+  match stuck_free 100 p icfg with
+  | ETerm (_, _, tobs) os =>
+      let (ids, mems) := split_sum_list tobs in
+      let leaked_vars := remove_dupes String.eqb ids in
+      checker (negb (existsb (String.eqb unused_var) leaked_vars))
+  | EOutOfFuel st os => checker tt
+  | EError st os => checker false
+  end)))).
+
+QuickChick unused_var_no_leak.
+(* +++ Passed 10000 tests (8072 discards) *)
+
+Definition test_ni `{Transform (prog * mem * reg)} := (
+  forAll (gen_prog_wt_with_basic_blk 3 8) (fun '(c, tm, pst, p) =>
+  forAll (gen_reg_wt c pst) (fun rs =>
+  forAll (gen_wt_mem tm pst) (fun m =>
+  let p := transform_load_store_prog c tm p in
+  let '(p, m, rs) := transform (p, m, rs) in
+  let icfg := (ipc, rs, m, istk) in
+  let r1 := taint_tracking 100 p icfg in
+  match r1 with
+  | Some (os1', tvars, tms) =>
+      let P := (false, map (fun x => (x,true)) tvars) in
+      let PM := tms_to_pm (Datatypes.length m) tms in
+      forAll (gen_pub_equiv_same_ty P rs) (fun rs' =>
+      forAll (gen_pub_mem_equiv_same_ty PM m) (fun m' =>
+      let (m', rs') := transform (m', rs') in
+      let icfg' := (ipc, rs', m', istk) in
+      let r2 := taint_tracking 100 p icfg' in
+      match r2 with
+      | Some (os2', _, _) => checker (obs_eqb os1' os2')
+      | None => checker false (* fail *)
+      end))
+   | None => checker tt (* discard *)
+  end)))).
+
+QuickChick test_ni.
+(* +++ Passed 10000 tests (0 discards) *)
+
+(* 
+  NOTE: This test
+  * generates MiniCET program
+  * transforms it to block-based Machine program
+  * runs speculative step on block-based Machine program
+*)
+
+Definition test_safety_preservation `{Show dir} `{Transform (prog * mem * reg)}
+  (gen_dbr : G dir) (gen_dcall : list nat -> G dir) := (
+  forAll (gen_prog_wt_with_basic_blk 3 8) (fun '(c, tm, pst, p) =>
+  forAll (gen_reg_wt c pst) (fun rs =>
+  forAll (gen_wt_mem tm pst) (fun m =>
+  let p := transform_load_store_prog c tm p in
+  let harden := uslh_prog p in
+  let '(harden, m, rs) := transform (harden, m, spec_rs rs) in
+  let icfg := (ipc, rs, m, istk) in
+  let iscfg := (icfg, true, false) in
+  let h_pst := pst_calc harden in
+  forAll (gen_spec_steps_sized 200 harden h_pst iscfg gen_dbr gen_dcall) (fun ods =>
+  (match ods with
+   | SETerm sc os ds => checker true
+   | SEError (c', _, _) _ ds => checker false
+   | SEOutOfFuel _ _ ds => checker tt
+   end))
+  )))).
+
+QuickChick (test_safety_preservation gen_dbr gen_dcall).
+(* +++ Passed 10000 tests (4236 discards) *)
+
+(* 
+  NOTE: This test
+  * generates MiniCET program
+  * transforms it to block-based Machine program
+  * runs speculative step on block-based Machine program
+*)
+
+Definition test_relative_security `{Show dir} `{Transform (prog * mem * reg)}
+  (gen_dbr : G dir) (gen_dcall : list nat -> G dir) := (
+  forAll (gen_prog_wt_with_basic_blk 3 8) (fun '(c, tm, pst, p) =>
+  forAll (gen_reg_wt c pst) (fun rs1 =>
+  forAll (gen_wt_mem tm pst) (fun m1 =>
+  let p := transform_load_store_prog c tm p in
+  let '(p, m1, rs1) := transform (p, m1, rs1) in
+  let icfg1 := (ipc, rs1, m1, istk) in
+  let r1 := taint_tracking 1000 p icfg1 in
+  match r1 with
+  | Some (os1', tvars, tms) =>
+      let P := (false, map (fun x => (x,true)) tvars) in
+      let PM := tms_to_pm (Datatypes.length m1) tms in
+      forAll (gen_pub_equiv_same_ty P rs1) (fun rs2 =>
+      forAll (gen_pub_mem_equiv_same_ty PM m1) (fun m2 =>
+      let icfg2 := (ipc, rs2, m2, istk) in
+      let r2 := taint_tracking 1000 p icfg2 in
+      match r2 with
+      | Some (os2', _, _) =>
+          if (obs_eqb os1' os2') (* The source program produces the same leakage for a pair of inputs. *)
+          then (let harden := uslh_prog p in
+                let rs1' := transform (spec_rs rs1) in
+                let icfg1' := (ipc, rs1', m1, istk) in
+                let iscfg1' := (icfg1', true, false) in
+                let h_pst := pst_calc harden in
+                forAll (gen_spec_steps_sized 1000 harden h_pst iscfg1' gen_dbr gen_dcall) (fun ods1 =>
+                (match ods1 with
+                 | SETerm _ os1 ds =>
+                     (* checker true *)
+                     let rs2' := transform (spec_rs rs2) in
+                     let icfg2' := (ipc, rs2', m2, istk) in
+                     let iscfg2' := (icfg2', true, false) in
+                     let sc_r2 := spec_steps_acc 1000 harden iscfg2' ds in
+                     match sc_r2 with
+                     | SETerm _ os2 _ => checker (obs_eqb os1 os2)
+                     | SEOutOfFuel _ _ _ => collect "se2 oof"%string (checker tt)
+                     | _ => collect "2nd speculative execution fails!"%string (checker tt) (* discard -- doesn't seem to happen *)
+                     end
+                 | SEOutOfFuel _ os1 ds => 
+                     let rs2' := transform (spec_rs rs2) in
+                     let icfg2' := (ipc, rs2', m2, istk) in
+                     let iscfg2' := (icfg2', true, false) in
+                     let sc_r2 := spec_steps_acc 1000 harden iscfg2' ds in
+                     match sc_r2 with
+                     | SETerm _ os2 _ => collect "se1 oof but se2 term"%string (checker tt) (* this would be very weird *)
+                     | SEOutOfFuel _ os2 _ => checker (obs_eqb os1 os2) (* equality should hold because essentially lockstep *)
+                     | _ => collect "2nd speculative execution fails!"%string (checker tt) (* discard -- doesn't seem to happen *)
+                     end
+                 | _ =>  collect "1st speculative execution fails!"%string (checker tt) (* discard -- doesn't seem to happen *)
+                 end))
+               )
+          else collect "seq obs differ"%string (checker tt) (* discard *)
+      | None => collect "tt2 failed"%string (checker tt) (* discard *)
+      end))
+   | None => collect "tt1 failed"%string (checker tt) (* discard *)
+  end)))).
+
+QuickChick (test_relative_security gen_dbr gen_dcall).
+(* +++ Passed 10000 tests (0 discards) *)
